RegexCorrectness/VM/CharStep.lean
@@ -1,4 +1,2 @@
-import RegexCorrectness.VM.CharStep.Path
-import RegexCorrectness.VM.CharStep.VMPath
 import RegexCorrectness.VM.CharStep.Basic
 import RegexCorrectness.VM.CharStep.Lemmas
