RegexCorrectness/VM/EpsilonClosure.lean
@@ -1,3 +1,2 @@
 import RegexCorrectness.VM.EpsilonClosure.Basic
-import RegexCorrectness.VM.EpsilonClosure.Path
 import RegexCorrectness.VM.EpsilonClosure.Lemmas
